tuning
* sharing some definitions theorems
* tune proofs

Weidenbach_Book/CDCL_Two_Watched_Literals_List_Watched_Code_Common.thy
@@ -1901,4 +1901,62 @@ qed
 
 end
 
+
+definition find_first_eq_map :: "('b \<Rightarrow> 'a) \<Rightarrow> 'a \<Rightarrow> 'b list \<Rightarrow> nat nres" where
+  \<open>find_first_eq_map f x xs = WHILE\<^sub>T\<^bsup>\<lambda>i. i \<le> length xs\<^esup>
+       (\<lambda>i. i < length xs \<and> f (xs!i) \<noteq> x)
+       (\<lambda>i. RETURN (i+1))
+       0\<close>
+
+lemma find_first_eq_map_index:
+  shows \<open>find_first_eq_map f x xs \<le> \<Down> nat_rel (RETURN (index (map f xs) x))\<close>
+proof -
+  have H:
+    \<open>WHILE\<^sub>T\<^bsup>\<lambda>i. i \<le> length xs\<^esup>
+       (\<lambda>i. i < length xs \<and> f (xs!i) \<noteq> x)
+       (\<lambda>i. RETURN (i+1))
+       k
+     \<le> \<Down> nat_rel
+       (RETURN (k + index (sublist (map f xs) {k..<length xs}) x))\<close>
+    if \<open>k < length xs\<close> for k
+    using that
+  proof (cases xs)
+    case Nil
+    then show ?thesis using that by simp
+  next
+    case xs: (Cons a xs')
+    have index_first: \<open>index (sublist (a # xs') {n..<Suc (length xs')}) ((a # xs') ! n) = 0\<close>
+      if \<open>n < length xs'\<close> for n
+      using that by (metis index_Cons length_Cons less_SucI sublist_upt_Suc)
+    have [simp]: "sublist (f a # map f xs') {n..<Suc (length xs')} =
+    (f a # map f xs') ! n # sublist (f a # map f xs') {Suc n..<Suc (length xs')}"
+      if a2: "n < length xs'" for n -- \<open>auto is not able to derive it automatically
+      because of @{thm length_Cons}\<close>
+      using a2
+      apply (subst length_Cons[of a, symmetric])+
+      apply (subst length_map[of f \<open>a # xs'\<close>, symmetric])+
+      by (metis length_Cons length_map less_SucI sublist_upt_Suc)
+    have [simp]: \<open>(f a # map f xs') ! n = f ((a # xs') ! n)\<close> if \<open>n < length (a#xs')\<close> for n
+      unfolding list.map[symmetric]
+      by (subst nth_map) (use that in auto)
+
+    have \<open>k < Suc (length xs')\<close>
+      using that xs by auto
+    then show ?thesis
+      unfolding find_first_eq_def less_eq_Suc_le Suc_le_mono xs
+      apply (induction rule: inc_induct)
+      subgoal by (auto simp: sublist_single_if WHILEIT_unfold )[]
+      subgoal by (subst WHILEIT_unfold) (auto simp: sublist_single_if index_first sublist_upt_Suc)
+      done
+  qed
+  have [simp]: \<open>find_first_eq_map f x [] \<le> RETURN 0\<close>
+    unfolding find_first_eq_map_def by (auto simp: WHILEIT_unfold)[]
+  have [simp]: \<open>sublist (map f xs) {0..<length xs} = map f xs\<close>
+    by (simp add: sublist_id_iff)
+  show ?thesis
+    apply (cases \<open>xs = []\<close>)
+     apply (solves simp)
+    using H[of 0] unfolding find_first_eq_map_def by simp
+qed
+
 end
